improved presentation

src/HOL/Auth/OtwayRees_AN.thy
@@ -25,33 +25,33 @@ From page 11 of
 consts  otway   :: "event list set"
 inductive "otway"
   intros
-         (*Initial trace is empty*)
-   Nil:  "[] \<in> otway"
+   Nil: --{*The empty trace*}
+        "[] \<in> otway"
 
-         (*The spy MAY say anything he CAN say.  We do not expect him to
-           invent new nonces here, but he can also use NS1.  Common to
-           all similar protocols.*)
-   Fake: "[| evsf \<in> otway;  X \<in> synth (analz (knows Spy evsf)) |]
+   Fake: --{*The Spy may say anything he can say.  The sender field is correct,
+            but agents don't use that information.*}
+         "[| evsf \<in> otway;  X \<in> synth (analz (knows Spy evsf)) |]
           ==> Says Spy B X  # evsf \<in> otway"
 
-         (*A message that has been sent can be received by the
-           intended recipient.*)
-   Reception: "[| evsr \<in> otway;  Says A B X \<in>set evsr |]
+        
+   Reception: --{*A message that has been sent can be received by the
+                  intended recipient.*}
+	      "[| evsr \<in> otway;  Says A B X \<in>set evsr |]
                ==> Gets B X # evsr \<in> otway"
 
-         (*Alice initiates a protocol run*)
-   OR1:  "evs1 \<in> otway
+   OR1:  --{*Alice initiates a protocol run*}
+         "evs1 \<in> otway
           ==> Says A B {|Agent A, Agent B, Nonce NA|} # evs1 \<in> otway"
 
-         (*Bob's response to Alice's message.*)
-   OR2:  "[| evs2 \<in> otway;
+   OR2:  --{*Bob's response to Alice's message.*}
+	 "[| evs2 \<in> otway;
              Gets B {|Agent A, Agent B, Nonce NA|} \<in>set evs2 |]
           ==> Says B Server {|Agent A, Agent B, Nonce NA, Nonce NB|}
                  # evs2 \<in> otway"
 
-         (*The Server receives Bob's message.  Then he sends a new
-           session key to Bob with a packet for forwarding to Alice.*)
-   OR3:  "[| evs3 \<in> otway;  Key KAB \<notin> used evs3;
+   OR3:  --{*The Server receives Bob's message.  Then he sends a new
+           session key to Bob with a packet for forwarding to Alice.*}
+	 "[| evs3 \<in> otway;  Key KAB \<notin> used evs3;
              Gets Server {|Agent A, Agent B, Nonce NA, Nonce NB|}
                \<in>set evs3 |]
           ==> Says Server B
@@ -59,18 +59,18 @@ inductive "otway"
                  Crypt (shrK B) {|Nonce NB, Agent A, Agent B, Key KAB|}|}
               # evs3 \<in> otway"
 
-         (*Bob receives the Server's (?) message and compares the Nonces with
-	   those in the message he previously sent the Server.
-           Need B \<noteq> Server because we allow messages to self.*)
-   OR4:  "[| evs4 \<in> otway;  B \<noteq> Server;
+   OR4:  --{*Bob receives the Server's (?) message and compares the Nonces with
+	     those in the message he previously sent the Server.
+             Need @{term "B \<noteq> Server"} because we allow messages to self.*}
+	 "[| evs4 \<in> otway;  B \<noteq> Server;
              Says B Server {|Agent A, Agent B, Nonce NA, Nonce NB|} \<in>set evs4;
              Gets B {|X, Crypt(shrK B){|Nonce NB,Agent A,Agent B,Key K|}|}
                \<in>set evs4 |]
           ==> Says B A X # evs4 \<in> otway"
 
-         (*This message models possible leaks of session keys.  The nonces
-           identify the protocol run.  B is not assumed to know shrK A.*)
-   Oops: "[| evso \<in> otway;
+   Oops: --{*This message models possible leaks of session keys.  The nonces
+             identify the protocol run.*}
+	 "[| evso \<in> otway;
              Says Server B
                       {|Crypt (shrK A) {|Nonce NA, Agent A, Agent B, Key K|},
                         Crypt (shrK B) {|Nonce NB, Agent A, Agent B, Key K|}|}
@@ -84,7 +84,7 @@ declare analz_into_parts [dest]
 declare Fake_parts_insert_in_Un  [dest]
 
 
-(*A "possibility property": there are traces that reach the end*)
+text{*A "possibility property": there are traces that reach the end*}
 lemma "[| B \<noteq> Server; Key K \<notin> used [] |]
       ==> \<exists>evs \<in> otway.
            Says B A (Crypt (shrK A) {|Nonce NA, Agent A, Agent B, Key K|})
@@ -102,9 +102,8 @@ lemma Gets_imp_Says [dest!]:
 by (erule rev_mp, erule otway.induct, auto)
 
 
-(**** Inductive proofs about otway ****)
 
-(** For reasoning about the encrypted portion of messages **)
+text{* For reasoning about the encrypted portion of messages *}
 
 lemma OR4_analz_knows_Spy:
      "[| Gets B {|X, Crypt(shrK B) X'|} \<in> set evs;  evs \<in> otway |]
@@ -112,14 +111,13 @@ lemma OR4_analz_knows_Spy:
 by blast
 
 
-(** Theorems of the form X \<notin> parts (knows Spy evs) imply that NOBODY
-    sends messages containing X! **)
+text{*Theorems of the form @{term "X \<notin> parts (spies evs)"} imply that
+NOBODY sends messages containing X! *}
 
-(*Spy never sees a good agent's shared key!*)
+text{*Spy never sees a good agent's shared key!*}
 lemma Spy_see_shrK [simp]:
      "evs \<in> otway ==> (Key (shrK A) \<in> parts (knows Spy evs)) = (A \<in> bad)"
-apply (erule otway.induct, simp_all, blast+)
-done
+by (erule otway.induct, simp_all, blast+)
 
 lemma Spy_analz_shrK [simp]:
      "evs \<in> otway ==> (Key (shrK A) \<in> analz (knows Spy evs)) = (A \<in> bad)"
@@ -130,9 +128,9 @@ lemma Spy_see_shrK_D [dest!]:
 by (blast dest: Spy_see_shrK)
 
 
-(*** Proofs involving analz ***)
+subsection{*Proofs involving analz *}
 
-(*Describes the form of K and NA when the Server sends this message.*)
+text{*Describes the form of K and NA when the Server sends this message.*}
 lemma Says_Server_message_form:
      "[| Says Server B
             {|Crypt (shrK A) {|NA, Agent A, Agent B, Key K|},
@@ -156,9 +154,9 @@ done
 ****)
 
 
-(** Session keys are not used to encrypt other session keys **)
+text{* Session keys are not used to encrypt other session keys *}
 
-(*The equality makes the induction hypothesis easier to apply*)
+text{*The equality makes the induction hypothesis easier to apply*}
 lemma analz_image_freshK [rule_format]:
  "evs \<in> otway ==>
    \<forall>K KK. KK <= -(range shrK) -->
@@ -176,8 +174,7 @@ lemma analz_insert_freshK:
 by (simp only: analz_image_freshK analz_image_freshK_simps)
 
 
-(*** The Key K uniquely identifies the Server's message. **)
-
+text{*The Key K uniquely identifies the Server's message.*}
 lemma unique_session_keys:
      "[| Says Server B
           {|Crypt (shrK A) {|NA, Agent A, Agent B, K|},
@@ -190,14 +187,13 @@ lemma unique_session_keys:
         evs \<in> otway |]
      ==> A=A' & B=B' & NA=NA' & NB=NB'"
 apply (erule rev_mp, erule rev_mp, erule otway.induct, simp_all)
-(*Remaining cases: OR3 and OR4*)
-apply blast+
+apply blast+  --{*OR3 and OR4*}
 done
 
 
-(**** Authenticity properties relating to NA ****)
+subsection{*Authenticity properties relating to NA*}
 
-(*If the encrypted message appears then it originated with the Server!*)
+text{*If the encrypted message appears then it originated with the Server!*}
 lemma NA_Crypt_imp_Server_msg [rule_format]:
     "[| A \<notin> bad;  A \<noteq> B;  evs \<in> otway |]
      ==> Crypt (shrK A) {|NA, Agent A, Agent B, Key K|} \<in> parts (knows Spy evs)
@@ -207,13 +203,12 @@ lemma NA_Crypt_imp_Server_msg [rule_format]:
                     \<in> set evs)"
 apply (erule otway.induct, force)
 apply (simp_all add: ex_disj_distrib)
-(*Fake, OR3*)
-apply blast+
+apply blast+  --{*Fake, OR3*}
 done
 
 
-(*Corollary: if A receives B's OR4 message then it originated with the Server.
-  Freshness may be inferred from nonce NA.*)
+text{*Corollary: if A receives B's OR4 message then it originated with the
+      Server. Freshness may be inferred from nonce NA.*}
 lemma A_trusts_OR4:
      "[| Says B' A (Crypt (shrK A) {|NA, Agent A, Agent B, Key K|}) \<in> set evs;
          A \<notin> bad;  A \<noteq> B;  evs \<in> otway |]
@@ -224,10 +219,9 @@ lemma A_trusts_OR4:
 by (blast intro!: NA_Crypt_imp_Server_msg)
 
 
-(** Crucial secrecy property: Spy does not see the keys sent in msg OR3
+text{*Crucial secrecy property: Spy does not see the keys sent in msg OR3
     Does not in itself guarantee security: an attack could violate
-    the premises, e.g. by having A=Spy **)
-
+    the premises, e.g. by having @{term "A=Spy"}*}
 lemma secrecy_lemma:
      "[| A \<notin> bad;  B \<notin> bad;  evs \<in> otway |]
       ==> Says Server B
@@ -239,9 +233,9 @@ lemma secrecy_lemma:
 apply (erule otway.induct, force)
 apply (frule_tac [7] Says_Server_message_form)
 apply (drule_tac [6] OR4_analz_knows_Spy)
-apply (simp_all add: analz_insert_eq analz_insert_freshK pushes, spy_analz)  (*Fake*)
-(*OR3, OR4, Oops*)
-apply (blast dest: unique_session_keys)+
+apply (simp_all add: analz_insert_eq analz_insert_freshK pushes)
+apply spy_analz  --{*Fake*}
+apply (blast dest: unique_session_keys)+  --{*OR3, OR4, Oops*}
 done
 
 
@@ -256,8 +250,8 @@ lemma Spy_not_see_encrypted_key:
 by (blast dest: Says_Server_message_form secrecy_lemma)
 
 
-(*A's guarantee.  The Oops premise quantifies over NB because A cannot know
-  what it is.*)
+text{*A's guarantee.  The Oops premise quantifies over NB because A cannot know
+  what it is.*}
 lemma A_gets_good_key:
      "[| Says B' A (Crypt (shrK A) {|NA, Agent A, Agent B, Key K|}) \<in> set evs;
          \<forall>NB. Notes Spy {|NA, NB, Key K|} \<notin> set evs;
@@ -267,10 +261,9 @@ by (blast dest!: A_trusts_OR4 Spy_not_see_encrypted_key)
 
 
 
-(**** Authenticity properties relating to NB ****)
+subsection{*Authenticity properties relating to NB*}
 
-(*If the encrypted message appears then it originated with the Server!*)
-
+text{*If the encrypted message appears then it originated with the Server!*}
 lemma NB_Crypt_imp_Server_msg [rule_format]:
  "[| B \<notin> bad;  A \<noteq> B;  evs \<in> otway |]
   ==> Crypt (shrK B) {|NB, Agent A, Agent B, Key K|} \<in> parts (knows Spy evs)
@@ -279,14 +272,13 @@ lemma NB_Crypt_imp_Server_msg [rule_format]:
                      Crypt (shrK B) {|NB, Agent A, Agent B, Key K|}|}
                    \<in> set evs)"
 apply (erule otway.induct, force, simp_all add: ex_disj_distrib)
-(*Fake, OR3*)
-apply blast+
+apply blast+  --{*Fake, OR3*}
 done
 
 
 
-(*Guarantee for B: if it gets a well-formed certificate then the Server
-  has sent the correct message in round 3.*)
+text{*Guarantee for B: if it gets a well-formed certificate then the Server
+  has sent the correct message in round 3.*}
 lemma B_trusts_OR3:
      "[| Says S B {|X, Crypt (shrK B) {|NB, Agent A, Agent B, Key K|}|}
            \<in> set evs;
@@ -298,7 +290,8 @@ lemma B_trusts_OR3:
 by (blast intro!: NB_Crypt_imp_Server_msg)
 
 
-(*The obvious combination of B_trusts_OR3 with Spy_not_see_encrypted_key*)
+text{*The obvious combination of @{text B_trusts_OR3} with 
+      @{text Spy_not_see_encrypted_key}*}
 lemma B_gets_good_key:
      "[| Gets B {|X, Crypt (shrK B) {|NB, Agent A, Agent B, Key K|}|}
           \<in> set evs;
